Does not peek past end (which implies cannot be grown by and does not eat into)

types.thy
@@ -704,4 +704,23 @@ lemma charset_not_in_c:
 
 
 
+\<comment> \<open>Characters that cannot extend\<close>
+(* Usable, for example, together with parser can parse print result and first_chars? *)
+definition char_cannot_extend :: "'a parser \<Rightarrow> char \<Rightarrow> bool" where
+  "char_cannot_extend p ch \<longleftrightarrow> (\<forall>c r l. has_result_ci p (c@l) c r l \<longrightarrow> has_result_ci p (c@(ch#l)) c r (ch#l))"
+
+definition does_not_peek_past_end :: "'a parser \<Rightarrow> bool" where
+  "does_not_peek_past_end p \<longleftrightarrow> (\<forall> c r l l'. has_result p (c@l) r l \<longrightarrow> has_result p (c@l') r l')"
+
+lemma no_peek_past_end_wf_stronger:
+  assumes "does_not_peek_past_end (parse A)"
+  assumes "bidef_well_formed A"
+  assumes "p_has_result (print A) i ipr"
+  shows "\<And>cs. has_result (parse A) (ipr@cs) i cs"
+  using assms[unfolded does_not_peek_past_end_def bidef_well_formed_def parser_can_parse_print_result_def]
+  apply auto
+  by (metis append.right_neutral)
+
+
+
 end
